my thoughts on formalizing saturation and semantic soundness

SystemFD/Metatheory/SemSoundness.lean
@@ -4,65 +4,159 @@ import SystemFD.Term.Variant
 import SystemFD.Metatheory.Canonicity
 import SystemFD.Metatheory.Confluence
 
+/-
 
-@[simp]
-def ShallowlyDeterm : Term -> Prop
-| .zero => false
-| .ctor2 .choice _ _ => false
-| _ => true
+Goal
+----
+
+We want to have a syntactic property P on terms of SystemFD
+(possibly indexed over types and context)
+st. the following holds for it:
+
+   P τ t ⇒
+   ∃ v, (t ⟶⋆ n) ∧
+        (Val Γ n ∧ v is confusion free)
+        ∨ n does not have a normal form
+
+The context Γ has to bear some responsibility for the term to be confusion free,
+as the · ⟶⋆ · relation is dependent on Γ for instantiating open methods. We call this
+property saturation. Intuitively, the saturation property enforces that the
+(well typed) open method call instantiations cannot cause confusion.
+
+To explicitly encode this property in our formalization:
+
+   SatCtx Γ ∧ P τ Γ t ⇒
+   ∃ v, (t ⟨Γ⟩⟶⋆ n) ∧
+        (Val Γ n ∧ v is confusion free)
+         ∨ n does not have a normal form
 
 
--- Shalowly Deterministic Value is a value which also shallowly deterministic
-@[simp]
-abbrev SDVal (Γ : Ctx Term) (t: Term) := Val Γ t ∧ ShallowlyDeterm t
+Confusion Free:
+---------------
+Take 1: A (well typed) term, t,
+is confusion free if for all term contexts C[⬝], and saturated context Γ
+C[t] ⟨Γ⟩ ⟶⋆ n s.t. n is a value and n does not contain open methods or `0 or ⊕ or guards
 
- -- where
--- |  SDVal :
---     Val Γ t ->
---     ShallowlyDeterm t ->
---     -- ¬ (ContainsVariant (Ctx.variants Γ) [.zero, .guard, .ctor2 .choice] t) ->
---     -- (∀ x, Term.Subexpr #x t -> Γ.is_openm x -> saturated Γ x) ->
---     SDVal Γ t
+Its definitely not the case that any C[⬝] would do.  Why?
+C[⬝] itself can easily induce confusion:
+if C[⬝] = 3 ⊕ ⬝ then any confusion free term results in confusion
+
+Idea:
+Apply some restriction on C[⬝].
+A term context C[⬝] is confusion free if it does not contain open methods, `0, ⊕ or guards
+The key observation is that confusion can be induced by only these 4 constructs.
+
+
+Take 2: A term is confusion free if in any confusion free term context  C[⬝], and a saturated context Γ
+C[t] ⟨Γ⟩ ⟶⋆ n s.t. n is a value (or it loops indefinitely) and n does not
+contain open methods or `0 or ⊕ or guards
+
+
+Context Saturation:
+-------------------
+Intuitively, a context Γ is saturated
+If for any open method in the context, there is only one instance that does not make the term vanish.
+
+Suppose `m` is the open method. with type ∀ τs. Qs ⇒ τ'
+now, consider all possible (well typed applications) of this open method.
+WLOG, `m [τs] ds` such that Γ ⊢ d : Q[α ↦ τ], Γ ⊢ m [τs] ds : τ'[α ↦ τ]
+
+now, `m` will have some associated instantiations I_j in the context of the form (Λ αs .guards ... )
+so `m [τs] ds` ⟶ (I_1 ⊕ I_2 ⊕ .. I_n) [τs] ds ⟶⋆ (I_1 [τs] ds) ⊕ (I_2 [τs] ds) ⊕ ... ⊕ (I_n [τs] ds)
+
+Now we want saturation property to capture the idea only one of these I_j survives.
+
+Take 1:
+    ∀ τs ds,
+      (τs are ground, ds are confusion free)
+    ∃ i, Γ d@ i = .inst #m t ∧ t [τs] ds - ̸⟶⋆ `0 ∧
+    ∀ k, k ≠ i ∧  Γ d@ k = .inst #m t' ∧ t' [τs] ds ⟶⋆ `0
+
+but our saturation property has too strict! ds shouldn't be confusion free, they can
+very well contain calls to open methods. This is where related inputs go to related outputs
+idea gets used (I think). ds should satisfy the original goal property P from above.
+
+Option: Let P be collection of terms that contains no guards, `0, ⊕. (open methods are okay)
+This seems to have some merit. It is a syntactic check and with context saturation ensuring no confusion
+
+Take 2:
+    ∀ τs ds,
+      (τs are ground, ds satisfy property P)
+    ∃ i, Γ d@ i = .inst #m t ∧ t [τs] ds - ̸⟶⋆ `0 ∧
+    ∀ k, k ≠ i,  Γ d@ k = .inst #m t' → (t' [τs] ds ⟶⋆ `0)
+
+-/
 
 
 namespace Term
 
 def mk_ty_tm_app (t : Term) (τs : List Term) (es : List Term) := (t.mk_ty_apps τs).mk_apps es
+notation:70 t:170 "⬝[" τs:170 "]⬝" es:170 "⬝" => mk_ty_tm_app t τs es
 
 -- Ground Types are the ones that are not lambda bound
-def GroundTy (Γ : Ctx Term) (t : Term) : Bool :=
-  sorry
+-- Int, Bool, Int → Bool, Maybe, Maybe Int are all ground types
+-- a → Int, Maybe a are not ground types
+def groundTy (Γ : Ctx Term) : Term -> Bool
+| #x => Γ.is_datatype x
+| (τ1 -t> τ2) => groundTy Γ τ1 && groundTy (.empty :: Γ) τ2
+| τ1 `@k τ2 => groundTy Γ τ1 && groundTy  Γ τ2
+| _ => false
 
 end Term
 
 
+namespace TermCtx
 
--- a. Semantically
+
+end TermCtx
+
+
+-- shallowly confusion free is a term that does not have a `0 or ⊕ at its head
+@[simp]
+abbrev ShallowlyConfusionFree (Γ : Ctx Term) : Term -> Prop
+| .zero => false
+| .ctor2 .choice _ _ => false
+| t => Term.isTerm Γ t
+
+
+-- Shalowly confusion free value is a value which also shallowly confusion free
+--   So, (λ x. `0) is a shallowly confusion free value.
+--   but  (`0  ⊕ `0) is not a shallowly confusion free value.
+@[simp]
+abbrev SCFVal (Γ : Ctx Term) (t: Term) := Val Γ t ∧ ShallowlyConfusionFree Γ t
+
+@[simp]
+abbrev CanCauseConfusion (Γ : Ctx Term) (t: Term) : Bool :=
+  Term.isTerm Γ t ∧
+  contains_variant Γ.variants [.var .openm, .zero, .guard, .ctor2 .choice] t
+
+
+-- a. Semantically,
 --    x is saturated iff
 --    ∀ τ e, x is open in Γ ->
 --    Val Γ e ->
 --    x[τ]e is of ground type ->
---    (∃ v, x[τ]e ⟶★ v ∧ SemWDVal Γ v)
+--    (∃ v, x[τ]e ⟶★ v ∧ Shallowly Confusion Free Γ v)
 @[simp]
-abbrev Sat (Γ : Ctx Term) (x : Nat):  Prop :=
-  Γ.is_openm x ∧
-  (∀ τs es,
-      (∀ e ∈ es, SDVal Γ e) ->
-      (∃ σ, Γ ⊢ (#x).mk_ty_tm_app τs es : σ ∧ σ.GroundTy Γ) ->
-      (∃ v, ((#x).mk_ty_tm_app τs es) ⟨ Γ ⟩⟶⋆ v ∧ SDVal Γ v))
+abbrev Sat (Wf : Ctx Term -> Term -> Prop)(Γ : Ctx Term) (x : Nat):  Prop :=
+  ⊢ Γ ∧
+  Γ.is_openm x ->
+  (∀ τs es σ,
+      (∀ τ ∈ τs, τ.groundTy Γ) ->
+      (∀ e ∈ es, Wf Γ e) ->
+      (Γ ⊢ (#x ⬝[ τs ]⬝ es ⬝) : σ ∧ σ.groundTy Γ ∧ ∃ k, Γ ⊢ σ : k ∧ Γ ⊢ k : □) ->
+      (∃ v, (#x ⬝[ τs ]⬝ es ⬝) ⟨ Γ ⟩⟶⋆ v ∧ Wf Γ v))
 
 @[simp]
-abbrev SatCtx (Γ : Ctx Term) : Prop := ∀ x, Γ.is_openm x -> Sat Γ x -- sorry
+-- if the variable is not an open thingy then it is automatically saturated
+abbrev SatCtx (Wf : Ctx Term -> Term -> Prop) (Γ : Ctx Term) : Prop := ∀ x, Γ.is_openm x -> Sat Wf Γ x
 
--- TODO: Change Term.subexpr to Term.contains_variant decidable predicate
+@[simp]
+-- A closed context is a context where there are only pure declarations and no let, lambda bound terms
+abbrev ClosedCtx (Γ : Ctx Term) : Prop :=
+  ⊢ Γ ∧  ∀ (x : Nat), (Γ d@ x).is_stable_red
 
--- Question: Is the term (λ x. `0) a value, is it weakly deterministic?
--- Claim: WD is a property of arbitrary terms.
--- We have normal forms:
--- Its shallowly determistic value if it doesn't have `0 or ⊕ at the head
---   So, (λ x. `0) is a shallowly deterministic value.
---   but  (`0  ⊕ `0) is not a shallowly deterministic value.
-
+-- Question: Is the term (λ x. `0) a value, but applying it to anything will make it vanish
 -- Weak Determinism is how we handle open methods
 -- this is where guards come in.
 -- in any context evaluation C, t is weakly deterministic
@@ -72,34 +166,34 @@ abbrev SatCtx (Γ : Ctx Term) : Prop := ∀ x, Γ.is_openm x -> Sat Γ x -- sorr
 -- Reductions do not preserve shallowness
 
 -- Semantic Characterization of a Weakly Deterministic Value
-inductive SemWDVal (Wf : Term -> Prop) (Γ : Ctx Term) : Term ->  Prop where
-| SemWDVal :
-    ¬ (ContainsVariant (Ctx.variants Γ) [.zero, .guard, .ctor2 .choice] t) ->
-    -- Complaint: this syntactic not semantic
+@[simp]
+abbrev CFVal (Wf : Term -> Prop) (t : Term): Prop := ∀ Γ,
+    -- ¬ (ContainsVariant (Ctx.variants Γ) [.zero, .guard, .ctor2 .choice] t) ∧
+    -- Complaint: this is syntactic not semantic
     -- (∀ x : Nat, Term.Subexpr #x t -> Γ.is_openm x -> (SemSat P Γ #x)) ->
-    -- (∃ v, t ⟨ Γ ⟩⟶⋆ v ∧ SemWDVal Wf Γ v) ->
-    SatCtx Γ ->
-    Wf t ->
-    SemWDVal Wf Γ t
+    -- (∃ v, t ⟨ Γ ⟩⟶⋆ v ∧ CFVal Wf Γ v) ->
+    ClosedCtx Γ ->
+    SatCtx ShallowlyConfusionFree Γ ->
+    Val Γ t ->
+    Wf t
 
--- IDEA1: fix this by marmaduking it
 
-inductive SemWDTerm (Γ : Ctx Term) : Term -> Prop where
+inductive CFTerm (Wf : Term -> Prop) (Γ : Ctx Term) : Term -> Prop where
 | WDBase :
-    (∃ v, (M ⟨ Γ ⟩⟶⋆ v) ∧  Val Γ v) ->
-    SemWDTerm Γ M
+    Wf M ->
+    CFTerm Wf Γ M
 | WDChoice1 :
-   SemWDTerm Γ M ->
+   CFTerm Wf Γ M ->
    (N ⟨ Γ ⟩⟶⋆ `0) ->
-   SemWDTerm Γ (M ⊕ N)
+   CFTerm Wf Γ (M ⊕ N)
 | WDChoice2 :
-   SemWDTerm Γ N ->
+   CFTerm Wf Γ N ->
    (M ⟨ Γ ⟩⟶⋆ `0) ->
-   SemWDTerm Γ (M ⊕ N)
+   CFTerm Wf Γ (M ⊕ N)
 
 -- chain
 theorem sanity :
-  SemWDTerm Γ M ->
+  CFTerm (λ M => ∃ v, (M ⟨ Γ ⟩⟶⋆ v) ∧ Val Γ v) Γ M ->
   ∃ v, (M ⟨ Γ ⟩⟶⋆ v) ∧ Val Γ v := by
 intro h;
 induction h
